chore: update to Lean v4.33.0-rc2

examples/Examples/ProgramsProofs/InstrumentedInsertionSort.lean
@@ -8,15 +8,15 @@ def insertSorted [Ord α] (arr : Array α) (i : Fin arr.size) : Array α :=
   | ⟨0, _⟩ => arr
   | ⟨i' + 1, _⟩ =>
     have : i' < arr.size := by
-      omega
+      grind
     match Ord.compare arr[i'] arr[i] with
     | .lt | .eq => arr
     | .gt =>
       have : (dbgTraceIfShared "array to swap" arr).size = arr.size := by
-        simp [dbgTraceIfShared]
+        grind [dbgTraceIfShared]
       insertSorted
         ((dbgTraceIfShared "array to swap" arr).swap i' i)
-        ⟨i', by simp [*]⟩
+        ⟨i', by grind [dbgTraceIfShared]⟩
 
 theorem insert_sorted_size_eq [Ord α] (len : Nat) (i : Nat) :
     (arr : Array α) → (isLt : i < arr.size) → (arr.size = len) →
@@ -26,15 +26,13 @@ theorem insert_sorted_size_eq [Ord α] (len : Nat) (i : Nat) :
     intro arr isLt hLen
     simp [insertSorted, *]
   | succ i' ih =>
-    intro arr isLt hLen
-    simp [insertSorted, dbgTraceIfShared]
-    split <;> simp [*]
+    grind [insertSorted, dbgTraceIfShared]
 
 def insertionSortLoop [Ord α] (arr : Array α) (i : Nat) : Array α :=
   if h : i < arr.size then
     have : (insertSorted arr ⟨i, h⟩).size - (i + 1) < arr.size - i := by
       rw [insert_sorted_size_eq arr.size i arr h rfl]
-      omega
+      grind
     insertionSortLoop (insertSorted arr ⟨i, h⟩) (i + 1)
   else
     arr
